Wasm_Assertions_Shallow.thy
@@ -1,0 +1,53 @@
+theory Wasm_Assertions_Shallow imports "WebAssembly/Wasm_Base_Defs" begin
+
+typedef lvar = "UNIV :: (nat) set" ..
+
+(* global, local, logical variables*)
+datatype var = Gl nat | Lc nat | Lv lvar
+
+(* variable store *)
+type_synonym var_st = "(var, v) map"
+
+definition var_st_locals :: "var_st \<Rightarrow> nat set" where
+  "var_st_locals st = {n. Lc n \<in> (dom st)}"
+
+definition var_st_globals :: "var_st \<Rightarrow> nat set" where
+  "var_st_globals st = {n. Gl n \<in> (dom st)}"
+
+(* abstract heap with max length *)
+type_synonym heap = "((nat, byte) map) \<times> (nat option)"
+
+(* local variable reification *)
+definition reifies_loc :: "[v list, var_st] \<Rightarrow> bool" where
+  "reifies_loc locs st \<equiv> \<forall>ln \<in> var_st_locals st. ln < (length locs) \<and> st (Lc ln) = Some (locs!ln)"
+
+(* global variable reification (with respect to a partial instance) *)
+definition reifies_glob :: "[global list, nat list, var_st] \<Rightarrow> bool" where
+  "reifies_glob gs igs st \<equiv>
+     \<forall>gn \<in> var_st_globals st.
+       gn < (length igs) \<and> igs!gn < (length gs) \<and> st (Gl gn) = Some (g_val (gs!(igs!gn)))"
+
+(* function reification (with respect to a partial instance) *)
+definition reifies_func :: "[cl list, nat list, cl list] \<Rightarrow> bool" where
+  "reifies_func cls icls fs \<equiv> list_all2 (\<lambda>icl f. icl < (length cls) \<and> cls!icl = f) icls fs"
+
+(* heap reification relations *)
+definition reifies_heap_contents :: "[mem, ((nat, byte) map)] \<Rightarrow> bool" where
+  "reifies_heap_contents m byte_m \<equiv>
+     \<forall>ind \<in> (dom byte_m). ind < mem_length m \<and> byte_m(ind) = Some (byte_at m ind)"
+
+definition reifies_heap_length :: "[mem, nat option] \<Rightarrow> bool" where
+  "reifies_heap_length m l_opt \<equiv> pred_option (\<lambda>l. mem_size m = l) l_opt"
+
+definition reifies_heap :: "[mem list, nat option, heap] \<Rightarrow> bool" where
+  "reifies_heap ms im_opt h \<equiv> let im = the im_opt in
+                               im < length ms
+                             \<and> reifies_heap_contents (ms!im) (fst h)
+                             \<and> reifies_heap_length (ms!im) (snd h)"
+
+(* store reification relation *)
+definition reifies_s :: "[s, inst, heap, var_st, cl list] \<Rightarrow> bool" where
+  "reifies_s s i h st fs \<equiv> reifies_glob (globs s) (inst.globs i) st
+                         \<and> reifies_func (funcs s) (inst.funcs i) fs
+                         \<and> reifies_heap (mem s) (inst.mem i) h"
+end
